Done with the proofs. Starting quickchick.

bft2.v
@@ -5,6 +5,7 @@ Require Import Coq.Logic.FunctionalExtensionality.
 Require Import Coq.Lists.List.
 Import ListNotations.
 Require Import Maps.
+Require Coq.omega.Omega.
 
 Definition ReplicaId := string.
 
@@ -21,16 +22,9 @@ Definition IsNonFaulty (r:Replica) :  Prop :=
 
 Print list.
 
-Inductive Message : Type := 
-| message: Replica -> nat -> Message.
+Definition State := list (Replica * (list nat)).
 
-Notation "<< r ; n >>" := (message r n).
-
-Inductive State : Type :=
-| prePrep: (Replica * (list Message)) -> State
-| prep : (Replica * (list Message)) -> State -> State.
-
-Definition ReplicaFun := State -> State.
+Definition ReplicaFun := nat -> State -> State.
 
 Definition nfrValue := 0.
 Definition faultyValue := 100.
@@ -38,47 +32,16 @@ Definition errorNotFound := 400.
 
 Fixpoint multicast (st:State) (v:nat) :=
   match st with
-  | prePrep (P, _)  => [<<P;v>>]
-  | prep (r, _) t => <<r;v>>::(multicast t v)
+  | nil  => nil
+  | (r, msgs)::t => (r, v::msgs)::(multicast t v)
   end.
 
-Definition getMsgVal msg := match msg with | message r v => v end.
-Definition getMsgReplica msg := match msg with | message r v => r end.
+Definition NFReplicaFun (msg:nat) (st:State) :=
+       multicast st msg.
 
 
-
-Fixpoint getPrePrepValue (st:State) :=
-  match st with
-    | prePrep (P, <<_; v>>::pPrepMsgs) => Some v
-    | prePrep (P, _) => None
-    | prep _ t => getPrePrepValue t
-    end.
-
-Inductive CliqState : State -> Prop :=
-| cliqPrePrep : forall (st:State),
-    ~((getPrePrepValue st) = None) -> CliqState st.
-
-Lemma prePrepValue_constant : forall st:State, CliqState st ->
-    forall (a:Replica) (msgs:list Message),
-       getPrePrepValue (st) = getPrePrepValue (prep (a, msgs) st).
-Admitted.
-
-Definition optVal (on : option nat) :=
- match on with
-  | None => faultyValue
-  | Some n => n
-  end.
-
-Definition NFReplicaFun (st:State) :=
-       prep (NFReplica, 
-            multicast (prep (NFReplica, nil) st) (optVal (getPrePrepValue st))) st.
-
-Compute (NFReplicaFun (prePrep (NFReplica, [<< NFReplica; 0 >>; << NFReplica; 0 >>]))).
-
-Definition FaultyReplicaFun (st:State) :=
-       prep (FaultyReplica, 
-              (multicast (prep (FaultyReplica, nil) st) faultyValue)) st.
-
+Definition FaultyReplicaFun (msg:nat) (st:State) :=
+       multicast st faultyValue.
 
 Definition GetReplicaFun (r:Replica) : ReplicaFun :=
   match r with
@@ -88,19 +51,6 @@ Definition GetReplicaFun (r:Replica) : ReplicaFun :=
 
 Definition System := list Replica.
 
-Fixpoint systemLen (sys:System) :=
-match sys with
-| nil => 0 
-| r::sys' => S (systemLen sys')
-end.
-
-Fixpoint stateLen (st:State) :=
-match st with
-    | prePrep (P, _) => 1
-    | prep (r, prepMsgs) t => S (stateLen t)
-    end.
-
-
 Fixpoint countNFR_system (sys:System) :=
 match sys with
   | nil => 0 
@@ -108,184 +58,84 @@ match sys with
   | FaultyReplica::sys' => countNFR_system sys'
 end.
 
+Definition F := 10.
+Definition CompleteSystem (sys:System) := length sys = 3*F+1 /\ countNFR_system sys = 2*F+1.
+Definition QuorumReq := 2*F+1.
+
+Definition initState (sys:list Replica) : State := ( (map (fun r => (r, nil)) sys)).
+Definition prePrep (sys:list Replica) := ( (map (fun r => nfrValue) sys)).
+Compute prePrep [FaultyReplica; NFReplica].
+
+Fixpoint ReplicateRequest (sys : System) (msg: list nat) (st : State):=
+match sys, msg with
+  | nil, nil => st
+  | (r::sys'), (m::mt) => (GetReplicaFun r) m (ReplicateRequest sys' mt st)
+  | _, _ => nil
+  end.
 
 Fixpoint countNFR_msgs msgs :=
 match msgs with
 | nil => 0
-| <<NFReplica;_>>::t => S (countNFR_msgs t)
-| _::t => countNFR_msgs t
+| v::t => if (beq_nat v nfrValue) then (S (countNFR_msgs t ))
+          else (countNFR_msgs t )
 end.
 
-Fixpoint countNFR_state (st:State) :=
+Fixpoint GatherCertificates (st:State) :=
 match st with
-  | prePrep (NFReplica, _) => 1
-  | prePrep _ => 0
-  | prep (NFReplica, _) t => S (countNFR_state t)
-  | prep _ t => countNFR_state t
+  | nil => nil
+  | (NFReplica, msgs)::t => (countNFR_msgs msgs)::(GatherCertificates t)
+  | _::t => GatherCertificates t
 end.
 
-Axiom sysLen : forall (sys : System), exists F:nat, systemLen sys = 3*F+1.
-Axiom sysNofNFR : forall (sys : System), exists F:nat, countNFR_system sys = 2*F+1.
-Axiom primaryNonFaulty : forall st:State, getPrePrepValue st = Some nfrValue.
-
-Fixpoint processRequestHelper (sys : System) (st : State) :=
-match sys with
-  | nil =>  st
-  | r::sys' => (GetReplicaFun r) (processRequestHelper sys' st) 
-  end.
-
-Definition initState sys := ( prePrep (NFReplica, (map (fun r => <<r ; nfrValue>>) (NFReplica::sys)))).
-
-Lemma multicast_length: forall (st1 st2 : State),
-    stateLen st1 = stateLen st2
-      -> forall v:nat, multicast st1 v = multicast st2 v.
-Admitted.
-
-Lemma processHelper_stLen : forall (sys : System) (st:State),
-    stateLen st = stateLen (processRequestHelper sys st).
-Admitted.
-
-Lemma ProcessRequest_NFR : forall (sys:System) (r : Replica),
-    IsNonFaulty r ->
-      forall st:State, st = initState (r::sys) ->
-      (processRequestHelper (r::sys) st) = 
-          (prep (r , (multicast (prep (NFReplica, nil) st) nfrValue)) 
-            (processRequestHelper sys st)).
-Proof. intros. destruct r.
-  - inversion H.
-  - simpl. unfold NFReplicaFun. simpl. rewrite primaryNonFaulty. simpl.
-      remember (processRequestHelper sys st) as st2. rewrite (multicast_length st st2).
-      reflexivity.
-      rewrite Heqst2; clear. apply processHelper_stLen.
-Qed.
-
-Definition ProcessRequest (sys : System) : State :=
-  processRequestHelper sys (initState sys).
-
-Lemma countNFR_IncNF : forall (sys:System) (r:Replica),
-    IsNonFaulty r ->
-    forall st:State, st = initState (r::sys) ->
-      countNFR_state (processRequestHelper (r::sys) st)
-          = S (countNFR_state (processRequestHelper sys st)).
-Proof. intros. destruct r.
-  - inversion H.
-  - reflexivity.
-Qed.
-
-Lemma stLen_sysLen : forall sys:System,
-      stateLen (ProcessRequest sys) = systemLen sys.
-Admitted.
-
-Fixpoint splitMsgs (msgs : list Message) :=
-match msgs with
+Fixpoint incCertificates (certs : list nat):=
+match certs with
 | nil => nil
-| m::t => [m] ++ (splitMsgs t)
+| h::t => (S h) :: (incCertificates t)
 end.
 
-Fixpoint groupMsgs (newMsgs : list Message) (tst : list (list Message)) :=
-match newMsgs, tst with
-| nil, nil => nil
-| m::mt , tstH :: tstT => (m::tstH)::(groupMsgs mt tstT)
-| _, _ => nil
-end.
-
-Fixpoint transposeState (st:State) :=
-match st with
-    | prePrep (P, prePrepMsgs) => [(splitMsgs prePrepMsgs)]
-    | prep (r, prepMsgs) t => groupMsgs prepMsgs (transposeState t)
-    end.
-
-
-Definition qc_incPrePrep ( occ : nat ) (oppv : option nat) :=
-  match oppv with
-  | Some n => if ( beq_nat n nfrValue) then
-                    (S occ)
-                else (occ)
-  | None => (occ)
-  end.
-
-Fixpoint countNFRValues (msgs:list Message) :=
-| match 
-
-(* Lemma forall i, replica i NF -> forall j, getMsgValueAtI = nfr. *)
-Definition countQuorumVotes (st' : State) (i:nat):=
-match st with
-    | prePrep _ (P, _) => S qc
-    | prep _ (r, prepMsgs) t => (GetQCertificate t i (qc_incPrePrep qc (getMsgValueAtI i prepMsgs)))
-    end.
-
-
-(* When the primary is correct, this should be the number of NF replicas in the system *)
-(* THIS is your connection to quorums *)
-Fixpoint GetQCertificate (st:State) (i:nat) (qc : nat) :=
-    
-
-Fixpoint getLedgersHelper (st originalSt : State) :=
-match st with
-| prePrep i (P, msgs) => [nfrValue]
-| prep i (NFReplica, _) t => (GetQCertificate originalSt i 0)::(getLedgersHelper t originalSt)
-| prep _ (FaultyReplica, _) t => getLedgersHelper t originalSt
-end.
-
-Definition assertQuorumAgreement (nVotes : nat):= Some(nfrValue).
-
-Definition GetLedgers (st:State) :=
-  map assertQuorumAgreement (getLedgersHelper st st).
-
-Inductive LedgerAgreement : (list (option nat)) -> Prop :=
-| empty_la : LedgerAgreement [(Some nfrValue)]
-| ind_la : forall (n: nat) (l : list (option nat)),
-            LedgerAgreement l -> 
-              (hd None l) = Some n ->
-                LedgerAgreement ((Some n)::l).
-
-Axiom CliqConnected : forall st:State, CliqState st.
-
-Lemma NFR_QCertificates : forall (i:nat) (sys:System),
-      GetQCertificate (NFReplicaFun i (ProcessRequest sys (S i))) i 0 = nfrValue.
-Admitted.
-
-Lemma NFR_ledger_nfrvalue:  
-        forall (sys:System) (r:Replica) (i:nat), 
-            IsNonFaulty r
-         -> (GetLedgers (ProcessRequest (replica r sys) i))
-            = (Some nfrValue)::(GetLedgers (ProcessRequest sys (S i))).
-Proof.
-  intros. induction r.
-    - inversion H.
-    - simpl. induction (ProcessRequest sys (S i)).
-      + simpl. unfold GetLedgers. destruct p. 
-        simpl. auto.
-      + simpl. destruct p. simpl. induction l.
-        { simpl.
-Admitted.
-
-
-
-Lemma FaultyR_ledger_novalue:  
-        forall (sys:System) (r:Replica) (i:nat), 
-            ~(IsNonFaulty r)
-         -> (GetLedgers (ProcessRequest (replica r sys) i))
-            = (GetLedgers (ProcessRequest sys i)).
-Admitted.
-
-Theorem StateValid : forall (sys : System),
-      forall i:nat, LedgerAgreement (GetLedgers (ProcessRequest sys i)).
-Proof. intros sys. induction sys.
-  - simpl. unfold GetLedgers. simpl. rewrite multicast_nv. constructor. 
-  - induction r.
-    + intros. rewrite FaultyR_ledger_novalue.
-        { simpl. apply IHsys. }
-        { auto. } 
-    + intros. rewrite NFR_ledger_nfrvalue.
-      { 
-        constructor. 
-        { apply IHsys. }
-        { induction (IHsys (S i)).
-          { reflexivity. }
-          { rewrite H in IHl. apply IHl. }
-        }
-      }
-      { reflexivity. }
+Lemma FaultyR_GatherCerts : forall (st:State) (m:nat),
+        GatherCertificates (FaultyReplicaFun m st) = GatherCertificates st.
+Proof. intros.
+  induction st.
+    - reflexivity.
+    - destruct a. destruct r; simpl; rewrite <- IHst; reflexivity.
 Qed.
 
+Lemma NFR_GatherCerts : forall (st:State),
+        GatherCertificates (NFReplicaFun nfrValue st) = incCertificates (GatherCertificates st).
+Proof. intros.
+   induction st.
+    - reflexivity.
+    - destruct a. destruct r.
+      + simpl. apply IHst.
+      + simpl. rewrite IHst. reflexivity.
+Qed.
+
+Inductive LedgerAgreement : (list nat) -> Prop :=
+| qcAgreement : forall (certs : list nat), 
+            Forall (fun x => ~ (lt x QuorumReq)) certs -> LedgerAgreement certs.
+
+Lemma IncCertificates_MaintainsLedger : forall (certs : list nat),
+      LedgerAgreement certs ->
+        LedgerAgreement (incCertificates certs).
+Proof. intros. induction H. constructor. induction certs.
+  - simpl. constructor.
+  - simpl. inversion H. constructor.
+    + admit.
+    + apply IHcerts. apply H3.
+Admitted. 
+
+Lemma StateValid : forall (sys:System) (st:State) (msgs:list nat),
+        CompleteSystem sys ->
+        st = (initState sys) /\ msgs = (prePrep sys) ->
+          LedgerAgreement (GatherCertificates (ReplicateRequest sys msgs st)).
+Proof.
+  intros sys. induction sys.
+    + intros. induction H. inversion H1.
+    + intros. induction H0. destruct a.
+      - simpl. rewrite H1. simpl. rewrite FaultyR_GatherCerts. apply IHsys.
+        { admit. } { split. admit. admit. }
+      - simpl. rewrite H1. simpl. rewrite NFR_GatherCerts. 
+        apply IncCertificates_MaintainsLedger. apply IHsys.
+        { admit. } { split. admit. admit. }
+Admitted.
